compiler/backend/proofs/flat_elimProofScript.sml
@@ -69,6 +69,12 @@ val findResultGlobals_def = Define `
 
 val findResultGlobals_ind = theorem "findResultGlobals_ind";
 
+val findSemPrimResGlobals_def = Define `
+    (findSemPrimResGlobals (Rerr e : (flatSem$v list, flatSem$v) semanticPrimitives$result) =
+       findResultGlobals (SOME e)) ∧
+    (findSemPrimResGlobals (Rval e) = findVglobalsL e)
+`
+
 (**************************** GLOBALS_REL *****************************)
 
 (* s = state, t = removed state *)
@@ -79,6 +85,31 @@ val globals_rel_def = Define `
         ⇒ EL n s.globals = EL n t.globals)
 `
 
+val globals_rel_refl = Q.store_thm("globals_rel_refl",
+    `∀ reachable s . globals_rel reachable s s`,
+    rw[globals_rel_def]
+);
+
+val globals_rel_trans = Q.store_thm("globals_rel_trans",
+    `∀ reachable s1 s2 s3 . 
+        globals_rel reachable s1 s2 ∧ globals_rel reachable s2 s3
+        ⇒ globals_rel reachable s1 s3`,
+    rw[globals_rel_def]
+);
+
+val globals_rel_sym = Q.store_thm("globals_rel_sym",
+    `∀ reachable s1 s2 . 
+        globals_rel reachable s1 s2 ⇔ globals_rel reachable s2 s1`,
+    rw[] >> EQ_TAC >> rw[globals_rel_def]
+);
+
+val globals_rel_equivalence = Q.store_thm("globals_rel_equivalence",
+    `∀ reachable . equivalence (globals_rel reachable)`,
+    rw[equivalence_def, reflexive_def, symmetric_def, transitive_def] >>
+    fs[globals_rel_sym, globals_rel_refl] >>
+    metis_tac[globals_rel_trans]
+);
+
 (**************************** DECSCLOSED *****************************)
 
 val decsClosed_def = Define `
@@ -87,18 +118,161 @@ val decsClosed_def = Define `
       (∀ n m . n ∈ domain reachable ∧ isReachable (mk_wf_set_tree t) n m 
       ⇒ m ∈ domain reachable)
 `
+(*** TO MOVE TO REACHABILITY THEORY ***)
+val union_num_set_sym = Q.store_thm ("union_num_set_sym",
+    `∀ t1:num_set t2 . union t1 t2 = union t2 t1`,
+    Induct >> fs[union_def] >> rw[] >> CASE_TAC >> fs[union_def]
+);
+
+val lookup_mk_wf_set_tree = Q.store_thm("lookup_mk_wf_set_tree",
+    `∀ n tree x . lookup n tree = SOME x ⇒ ∃ y . lookup n (mk_wf_set_tree tree) = SOME y ∧ domain x = domain y`,
+    rw[flat_elimTheory.mk_wf_set_tree_def] >> rw[lookup_map] >> rw[lookup_union]
+);
+
+val num_set_tree_union_sym = Q.store_thm("num_set_tree_union_sym",
+    `∀ (t1 : num_set num_map) t2 . num_set_tree_union t1 t2 = num_set_tree_union t2 t1`,
+    Induct >> rw[num_set_tree_union_def] >> Cases_on `t2` >> fs[num_set_tree_union_def] >>
+    fs[union_num_set_sym]
+);
+
+val lookup_domain_num_set_tree_union = Q.store_thm("lookup_domain_num_set_tree_union",
+    `∀ n (t1:num_set num_map) t2 x . lookup n t1 = SOME x 
+    ⇒ ∃ y . lookup n (num_set_tree_union t1 t2) = SOME y ∧ domain x ⊆ domain y`,
+    Induct_on `t1` >> rw[] 
+    >- fs[lookup_def]
+    >- (fs[lookup_def, num_set_tree_union_def] >> CASE_TAC >> fs[lookup_def, domain_union])
+    >- (fs[lookup_def, num_set_tree_union_def] >> CASE_TAC >> fs[lookup_def, domain_union] >>
+        Cases_on `EVEN n` >> fs[])
+    >- (fs[lookup_def, num_set_tree_union_def] >> CASE_TAC >> fs[lookup_def, domain_union] >>
+        Cases_on `n = 0` >> fs[domain_union] >> Cases_on `EVEN n` >> fs[])
+);
+
+val lookup_NONE_num_set_tree_union = Q.store_thm ("lookup_NONE_num_set_tree_union",
+    `∀ n (t1:num_set num_map) t2 . lookup n t1 = NONE
+    ⇒ lookup n (num_set_tree_union t1 t2) = lookup n t2`,
+    Induct_on `t1` >> rw[] >> fs[lookup_def, num_set_tree_union_def] >>
+    Cases_on `t2` >> fs[lookup_def] >> Cases_on `n = 0` >> fs[] >>
+    Cases_on `EVEN n` >> fs[]
+);
+
+val lookup_SOME_SOME_num_set_tree_union = Q.store_thm ("lookup_SOME_SOME_num_set_tree_union",
+    `∀ n (t1:num_set num_map) x1 t2 x2 . lookup n t1 = SOME x1 ∧ lookup n t2 = SOME x2
+    ⇒ lookup n (num_set_tree_union t1 t2) = SOME (union x1 x2)`,
+    Induct_on `t1` >> rw[] >> fs[lookup_def, num_set_tree_union_def] >>
+    Cases_on `t2` >> fs[lookup_def] >>
+    Cases_on `EVEN n` >> fs[] >>
+    Cases_on `n = 0` >> fs[]
+);
+
+val lookup_num_set_tree_union = Q.store_thm("lookup_num_set_tree_union",
+    `∀ (t1 : num_set num_map) t2 n . 
+        lookup n (num_set_tree_union t1 t2) = case (lookup n t1) of
+            | NONE => lookup n t2
+            | SOME s1 => case (lookup n t2) of 
+                | NONE => SOME s1 
+                | SOME s2 => SOME (union s1 s2)`,
+    rw[] >> Cases_on `lookup n t1` >> fs[]
+    >-  fs[lookup_NONE_num_set_tree_union] 
+    >- (Cases_on `lookup n t2` >> fs[]
+        >- (fs[lookup_NONE_num_set_tree_union, num_set_tree_union_sym] >>
+            imp_res_tac lookup_NONE_num_set_tree_union >>
+            pop_assum (qspec_then `t1` mp_tac) >> rw[] >>
+            fs[num_set_tree_union_sym])
+        >-  fs[lookup_SOME_SOME_num_set_tree_union])
+);
+                
+val isAdjacent_num_set_tree_union = Q.store_thm("isAdjacent_num_set_tree_union",
+    `∀ t1 t2 n m . 
+        isAdjacent t1 n m ⇒ isAdjacent (num_set_tree_union t1 t2) n m`,
+    rw[isAdjacent_def] >> imp_res_tac lookup_domain_num_set_tree_union >>
+    first_x_assum (qspec_then `t2` mp_tac) >> rw[] >> 
+    first_x_assum (qspec_then `t2` mp_tac) >> rw[] >>
+    fs[SUBSET_DEF, domain_lookup]
+);
+
+val lookup_domain_mk_wf_set_tree = Q.store_thm("lookup_domain_mk_wf_set_tree",
+    `∀ n t x y . lookup n (mk_wf_set_tree t) = SOME x ⇒
+        lookup n t = SOME y ⇒ domain y = domain x`,
+    rw[flat_elimTheory.mk_wf_set_tree_def] >> fs[lookup_map, lookup_union] >>
+    metis_tac[domain_mk_wf]
+);
+
+val superdomain_inverse_thm = Q.store_thm("superdomain_inverse_thm",
+    `∀ n tree . n ∈ domain (superdomain tree) 
+    ⇒ ∃ k aSet . lookup k tree = SOME aSet ∧ n ∈ domain aSet`,
+    Induct_on `tree` >> rw[superdomain_def] >> fs[lookup_def, domain_union] >> res_tac
+    >- (qexists_tac `2 * k + 2` >> fs[EVEN_DOUBLE, EVEN_ADD] >> once_rewrite_tac[MULT_COMM] >> fs[DIV_MULT])
+    >- (qexists_tac `2 * k + 1` >> fs[EVEN_DOUBLE, EVEN_ADD] >> once_rewrite_tac[MULT_COMM] >> fs[MULT_DIV])
+    >- (qexists_tac `2 * k + 2` >> fs[EVEN_DOUBLE, EVEN_ADD] >> once_rewrite_tac[MULT_COMM] >> fs[DIV_MULT])
+    >- (qexists_tac `0` >> fs[])
+    >- (qexists_tac `2 * k + 1` >> fs[EVEN_DOUBLE, EVEN_ADD] >> once_rewrite_tac[MULT_COMM] >> fs[MULT_DIV])
+);
+
+val superdomain_not_in_thm = Q.store_thm("superdomain_not_in_thm",
+    `∀ n tree . n ∉ domain (superdomain tree) ⇒ ∀ k aSet . lookup k tree = SOME aSet ⇒ n ∉ domain aSet`,
+    Induct_on `tree` >> rw[superdomain_def] >> fs[lookup_def, domain_union] >> res_tac >>
+    Cases_on `k = 0` >> Cases_on `EVEN k` >> fs[] >> metis_tac[]
+);
+
+val domain_superdomain_num_set_tree_union = Q.store_thm("domain_superdomain_num_set_tree_union",
+    `∀ t1 t2 . domain (superdomain t1) ⊆ domain (superdomain (num_set_tree_union t1 t2))`,
+    fs[SUBSET_DEF] >> rw[] >> imp_res_tac superdomain_inverse_thm >> 
+    imp_res_tac lookup_domain_num_set_tree_union >> pop_assum (qspec_then `t2` mp_tac) >>
+    rw[] >> imp_res_tac superdomain_thm >> metis_tac[SUBSET_DEF]
+);
+
+val isAdjacent_wf_set_tree_num_set_tree_union = Q.store_thm ("isAdjacent_wf_set_tree_num_set_tree_union",
+    `∀ t1 t2 n m . 
+        isAdjacent (mk_wf_set_tree t1) n m 
+        ⇒ isAdjacent (mk_wf_set_tree (num_set_tree_union t1 t2)) n m`,
+    rw[isAdjacent_def] >> fs[mk_wf_set_tree_def] >> fs[lookup_map] >> 
+    fs[lookup_union] >> fs[lookup_map] >> fs[PULL_EXISTS] >> fs[lookup_num_set_tree_union] >>
+    Cases_on `lookup n t1` >> fs[] >> Cases_on `lookup n t2` >> fs[] >>
+    rveq >> fs[lookup_def, mk_wf_def, lookup_union] >> EVERY_CASE_TAC >> fs[] >>
+    qspecl_then [`t1`, `t2`] mp_tac domain_superdomain_num_set_tree_union >>
+    rw[SUBSET_DEF, domain_lookup]
+);
+
+(*
+val mk_wf_set_tree_num_set_tree_union = Q.store_thm("mk_wf_set_tree_num_set_tree_union",
+    `∀ t1 t2 . mk_wf_set_tree (num_set_tree_union t1 t2) = 
+        num_set_tree_union (mk_wf_set_tree t1) (mk_wf_set_tree t2)`,
+    rw[] >>
+    `wf (mk_wf_set_tree (num_set_tree_union t1 t2))` by metis_tac[mk_wf_set_tree_thm, wf_set_tree_def] >>
+    `wf (num_set_tree_union (mk_wf_set_tree t1) (mk_wf_set_tree t2))` by 
+        metis_tac[mk_wf_set_tree_thm, wf_set_tree_def, wf_num_set_tree_union] >> 
+    rw[spt_eq_thm] >>
+    simp[mk_wf_set_tree_def] >>
+    fs[lookup_map] >> fs[lookup_union] >> fs[lookup_map] >>
+    fs[lookup_num_set_tree_union] >>
+    fs[lookup_map] >> fs[lookup_union] >>
+    fs[lookup_map] >> fs[OPTION_MAP_COMPOSE, mk_wf_def] >>
+    Cases_on `lookup n t1` >> Cases_on `lookup n t2` >> fs[] >>
+    EVERY_CASE_TAC >> fs[mk_wf_def, union_def] >>
+    
+    `lookup n (num_set_tree_union t1 t2) = NONE` by fs[lookup_num_set_tree_union] >>
+
+cheat (* TODO - not necessary for now, but a useful result *)
+);
+*)
+
+val isReachable_wf_set_tree_num_set_tree_union = Q.store_thm ("isReachable_wf_set_tree_num_set_tree_union",
+    `∀ t1 t2 n m . 
+        isReachable (mk_wf_set_tree t1) n m ⇒ isReachable (mk_wf_set_tree (num_set_tree_union t1 t2)) n m`,
+    simp[isReachable_def] >> strip_tac >> strip_tac >> 
+    ho_match_mp_tac RTC_INDUCT_RIGHT1 >> rw[] >>
+    simp[Once RTC_CASES2] >> disj2_tac >> qexists_tac `m` >> fs[] >> 
+    imp_res_tac isAdjacent_wf_set_tree_num_set_tree_union >> fs[]
+); 
 
 val decsClosed_reduce = Q.store_thm ("decsClosed_reduce",
     `∀ reachable h t . decsClosed reachable (h::t) ⇒ decsClosed reachable t`,
     fs[decsClosed_def] >> rw[] >> Cases_on `h` >> fs[analyseCode_def] 
     >- (Cases_on `analyseExp e` >> fs[codeAnalysis_union_def, domain_union])
-    >- (
-        Cases_on `analyseExp e` >> fs[codeAnalysis_union_def, domain_union] >>
-        first_x_assum drule >> rw[] >>
-        pop_assum match_mp_tac >>
-        fs[isReachable_def] >>
-        cheat (* TODO *)
-    )
+    >- (Cases_on `analyseExp e` >> fs[codeAnalysis_union_def, domain_union] >>
+        first_x_assum drule >> rw[] >> pop_assum match_mp_tac >>
+        assume_tac isReachable_wf_set_tree_num_set_tree_union >> fs[] >>
+        fs[Once num_set_tree_union_sym])
     >> metis_tac[] 
 );
 
@@ -112,6 +286,17 @@ val flat_state_rel_def = Define `
     domain (findRefsGlobals s.refs) ⊆ domain reachable
 `
 
+val flat_state_rel_trans = Q.store_thm("flat_state_rel_trans",
+    `∀ reachable s1 s2 s3 . flat_state_rel reachable s1 s2 ∧ flat_state_rel reachable s2 s3 
+    ⇒ flat_state_rel reachable s1 s3`,
+    rw[flat_state_rel_def, globals_rel_def]
+);
+
+val flat_state_rel_triangle = Q.store_thm("flat_state_rel_triangle",
+    `∀ reachable s1 s2 s3 . flat_state_rel reachable s1 s2 ∧ flat_state_rel reachable s1 s3 
+    ⇒ flat_state_rel reachable s2 s3`,
+    rw[flat_state_rel_def, globals_rel_def] >> metis_tac[]
+);
 
 (******************************************************** OTHER LEMMAS *********************************************************)
 
@@ -125,10 +310,188 @@ val keep_Dlet = Q.store_thm("keep_Dlet",
 
 (******************************************************** MAIN PROOFS *********************************************************)
 
+val evaluate_sing_keep_flat_state_rel_eq = Q.store_thm("evaluate_sing_keep_flat_state_rel_eq",
+    `(∀ env (state:'ffi flatSem$state) exprL new_state result expr reachable removed_state . 
+        flatSem$evaluate (env with v := []) state exprL = (new_state, result) ∧ exprL = [expr] ∧ 
+        keep reachable (Dlet expr) ∧ 
+        flat_state_rel reachable state removed_state ∧ 
+        domain (findEnvGlobals env) ⊆ domain reachable ∧  
+        result ≠ Rerr (Rabort Rtype_error)
+    ⇒ ∃ new_removed_state . 
+        evaluate (env with v := []) removed_state exprL = (new_removed_state, result) ∧
+        flat_state_rel reachable new_state new_removed_state ∧ 
+        domain (findSemPrimResGlobals result) ⊆ domain reachable)
+  ∧ 
+    (∀ env (state:'ffi flatSem$state) v patExp_list err_v new_state result reachable removed_state .
+        evaluate_match (env with v := []) state v patExp_list err_v = (new_state, result) ∧
+        flat_state_rel reachable new_state removed_state ∧
+        domain (findEnvGlobals env) ⊆ domain reachable ∧ 
+        result ≠ Rerr (Rabort Rtype_error)
+    ⇒ ∃ new_removed_state .
+        evaluate_match (env with v := []) removed_state v patExp_list err_v = (new_removed_state, result) ∧ 
+        flat_state_rel reachable new_state new_removed_state ∧ 
+        domain (findSemPrimResGlobals result) ⊆ domain reachable)`
+  ,
+    ho_match_mp_tac evaluate_ind >> rw[] >>
+    qpat_assum `flat_state_rel _ _ _` mp_tac >> 
+    SIMP_TAC std_ss [Once flat_state_rel_def] >> strip_tac
+    (* 14 subgoals *)
+    >| [
+        qpat_x_assum `evaluate _ _ _ = _` mp_tac >>
+        simp[flatSemTheory.evaluate_def] >> 
+        rw[] >> fs[findSemPrimResGlobals_def, findVglobals_def]
+      , 
+        qpat_x_assum `evaluate _ _ _ = _` mp_tac >> simp[flatSemTheory.evaluate_def] >>
+        Cases_on `evaluate (env with v:=[]) state' [e]` >> fs[] >>
+        first_x_assum (qspecl_then [`reachable`, `removed_state`] mp_tac) >>
+        rw[] >> fs[keep_def] >> qpat_x_assum `inter _ _ ≠ _` mp_tac >> 
+        simp[Once findLoc_def] >> strip_tac >> fs[] >> rfs[] >>
+        `r ≠ Rerr (Rabort Rtype_error)` by (CCONTR_TAC >> Cases_on `r` >> fs[]) >>
+        fs[] >> Cases_on `r` >> fs[] >> rveq >> 
+        fs[findSemPrimResGlobals_def, findResultGlobals_def] >>
+        `LENGTH a = 1` by (imp_res_tac evaluate_length >> fs[LENGTH]) >>
+        Cases_on `a` >> fs[findVglobals_def]
+      ,
+        qpat_x_assum `evaluate _ _ _ = _` mp_tac >> simp[flatSemTheory.evaluate_def] >>
+        Cases_on `evaluate (env with v:=[]) state' [e]` >> fs[] >>
+        first_x_assum (qspecl_then [`reachable`, `removed_state`] mp_tac) >>
+        rw[] >> fs[keep_def] >> qpat_x_assum `inter _ _ ≠ _` mp_tac >> 
+        simp[Once findLoc_def] >> strip_tac >> fs[] >> rfs[] >>
+        `inter (findLoc e) reachable ≠ LN` by cheat (* TODO *) >> 
+        `r ≠ Rerr (Rabort Rtype_error)` by (CCONTR_TAC >> Cases_on `r` >> fs[]) >>
+        fs[] >> rfs[] >>
+        Cases_on `r` >> fs[] >> rveq >>
+        Cases_on `e'` >> fs[] >>
+        cheat (* TODO *)
+      ,
+      cheat,
+      cheat,
+      cheat,
+      cheat,
+      cheat,
+      cheat,
+      cheat,
+      cheat,
+      cheat,
+      cheat,
+      cheat
+
+    ]    
+);
+
+val evaluate_dec_flat_state_rel = Q.store_thm("evaluate_dec_state_rel",
+    `∀ env (state:'ffi flatSem$state) dec new_state new_ctors result reachable removed_state . 
+        evaluate_dec env state dec = (new_state, new_ctors, result) ∧ 
+        flat_state_rel reachable state removed_state ∧ keep reachable dec ∧
+        result ≠ SOME (Rabort Rtype_error) ∧ 
+        domain (findEnvGlobals env) ⊆ domain reachable
+    ⇒ ∃ new_removed_state . 
+        evaluate_dec env removed_state dec = (new_removed_state, new_ctors, result) ∧ 
+        flat_state_rel reachable new_state new_removed_state ∧ 
+        domain (findResultGlobals result) ⊆ domain reachable`
+      ,
+        rw[] >> qpat_x_assum `evaluate_dec _ _ _ = _` mp_tac >> 
+        reverse(Induct_on `dec`) >> fs[evaluate_dec_def] >> strip_tac >> strip_tac >>
+        fs[keep_def] 
+        >- (reverse(Cases_on `env.check_ctor`) >> fs[is_fresh_exn_def] >>
+            rw[] >> fs[findResultGlobals_def])
+        >- (reverse(Cases_on `env.check_ctor`) >> fs[is_fresh_exn_def] >>
+            rw[] >> fs[findResultGlobals_def])
+        >- (assume_tac evaluate_sing_keep_flat_state_rel_eq >> fs[] >>
+            pop_assum kall_tac >>
+            Cases_on `evaluate (env with v := []) state' [e]` >> fs[] >>
+            first_x_assum (qspecl_then [`env`, `state'`, `q`, `r`, `e`, 
+                `reachable`, `removed_state`] mp_tac) >> strip_tac >>
+            fs[keep_def] >> rfs[] >>
+            strip_tac >>
+            `r ≠ Rerr (Rabort Rtype_error)` by (CCONTR_TAC >> Cases_on `r` >> fs[]) >>
+            qpat_x_assum `_ = (_,_,_) ` mp_tac >> fs[] >>
+            EVERY_CASE_TAC >> fs[] >> rw[] >> fs[findResultGlobals_def, findSemPrimResGlobals_def])
+);
+
+val evaluate_sing_notKeep_flat_state_rel = Q.store_thm("evaluate_sing_notKeep_state_rel",
+    `(∀ env (state:'ffi flatSem$state) exprL new_state result expr reachable removed_state . 
+        flatSem$evaluate (env with v := []) state exprL = (new_state, result) ∧ exprL = [expr] ∧ 
+        ¬keep reachable (Dlet expr) ∧ 
+        flat_state_rel reachable state removed_state ∧ 
+        domain (findEnvGlobals env) ⊆ domain reachable ∧  
+        result ≠ Rerr (Rabort Rtype_error)
+    ⇒ flat_state_rel reachable new_state removed_state ∧ ∃ value : flatSem$v . result = Rval [value] ∧
+      domain (findVglobals value) ⊆ domain reachable)
+  ∧ 
+    (∀ env (state:'ffi flatSem$state) v patExp_list err_v new_state result reachable removed_state .
+        evaluate_match (env with v := []) state v patExp_list err_v = (new_state, result) ∧
+        (*¬ keep reachable (Dlet XXXXX) ∧*)
+        flat_state_rel reachable new_state removed_state ∧
+        domain (findEnvGlobals env) ⊆ domain reachable ∧ 
+        result ≠ Rerr (Rabort Rtype_error)
+    ⇒ flat_state_rel reachable new_state removed_state ∧ ∃ value : flatSem$v . result = Rval [value] ∧ 
+      domain (findVglobals value) ⊆ domain reachable)`
+,
+    ho_match_mp_tac evaluate_ind >> rw[] >>
+    qpat_assum `flat_state_rel _ _ _` mp_tac >> 
+    SIMP_TAC std_ss [Once flat_state_rel_def] >> strip_tac
+    
+    (* 26 subgoals - 13 flatLang expressions, two conjuncts in goal for each *)
+    >| [
+        qpat_x_assum `evaluate _ _ _ = _` mp_tac >>
+        simp[flatSemTheory.evaluate_def] >> rw[] >> fs[]
+    ,
+        qpat_x_assum `evaluate _ _ _ = _` mp_tac >>
+        simp[flatSemTheory.evaluate_def] >> rw[] >> fs[findVglobals_def]
+    ,
+        qpat_x_assum `evaluate _ _ _ = _` mp_tac >>
+        simp[flatSemTheory.evaluate_def] >>
+        Cases_on `evaluate (env with v := []) state' [e]` >> fs[] >>
+        first_x_assum (qspecl_then [`reachable`, `removed_state`] mp_tac) >>
+        fs[keep_def, Once findLoc_def] >> rw[] >>
+        `r ≠ Rerr (Rabort Rtype_error)` by (CCONTR_TAC >> Cases_on `r` >> fs[]) >>
+        fs[] >> Cases_on `r` >> fs[]
+    ,   
+        qpat_x_assum `evaluate _ _ _ = _` mp_tac >>
+        simp[flatSemTheory.evaluate_def] >>
+        Cases_on `evaluate (env with v := []) state' [e]` >> fs[] >>
+        first_x_assum (qspecl_then [`reachable`, `removed_state`] mp_tac) >>
+        rw[] >>
+        fs[keep_def, Once findLoc_def] >> rw[] >>
+        Cases_on `r` >> fs[] >>
+        rveq >> fs[] >>
+        cheat (* TODO - DOESN'T SEEM TO BE TRUE *)
+    ,
+        qpat_x_assum `evaluate _ _ _ = _` mp_tac >> simp[flatSemTheory.evaluate_def] >>
+        Cases_on `evaluate (env with v := []) state' [e]` >> fs[] >>
+        cheat (* TODO *)
+    ,
+        cheat,
+        cheat,
+        cheat,
+        cheat,
+        cheat,
+        cheat,
+        cheat,
+        cheat,
+        cheat,
+        cheat,
+        cheat,
+        cheat,
+        cheat,
+        cheat,
+        cheat,
+        cheat,
+        cheat,
+        cheat,
+        cheat,
+        cheat,
+        cheat
+    ]
+);
+
+
+
 (**************************** FLAT_DECS_REMOVAL LEMMA *****************************)
 
 val flat_decs_removal_lemma = Q.store_thm ("flat_decs_removal_lemma",
-    `∀ env state decs new_state new_ctors result reachable removed_decs removed_state . 
+    `∀ env (state:'ffi flatSem$state) decs new_state new_ctors result reachable removed_decs removed_state . 
         evaluate_decs env state decs = (new_state, new_ctors, result) ∧ 
         result ≠ SOME (Rabort Rtype_error) ∧ 
         removeUnreachable reachable decs = removed_decs ∧
@@ -139,46 +502,34 @@ val flat_decs_removal_lemma = Q.store_thm ("flat_decs_removal_lemma",
         evaluate_decs env removed_state removed_decs = (new_removed_state, new_ctors, result) ∧
         flat_state_rel reachable new_state new_removed_state ∧ 
         domain (findResultGlobals result) ⊆ domain reachable`
-,cheat); (* 
+  ,
     Induct_on `decs` 
     >- (rw[evaluate_decs_def, removeUnreachable_def] >> fs[evaluate_decs_def, findResultGlobals_def])
-    >> fs[evaluate_decs_def, removeUnreachable_def] >> reverse(rw[])
+    >>  fs[evaluate_decs_def, removeUnreachable_def] >> rw[] >>
+        qpat_assum `flat_state_rel _ _ _` mp_tac >> SIMP_TAC std_ss [Once flat_state_rel_def] >> strip_tac
+        >- (fs[evaluate_decs_def] >> `∃ r . evaluate_dec env state' h = r` by simp[] >> 
+            PairCases_on `r` >> fs[] >> `r2 ≠ SOME (Rabort Rtype_error)` by (CCONTR_TAC >> fs[]) >> 
+            drule evaluate_dec_flat_state_rel >> rpt (disch_then drule) >> rw[] >> fs[] >> 
+            Cases_on `r2` >> fs[] >> rw[] >> EVERY_CASE_TAC >> first_x_assum drule >> fs[] >> 
+            rveq >> disch_then drule >> reverse(impl_tac) >- rw[] >> fs[findEnvGlobals_def] >>
+            imp_res_tac decsClosed_reduce)
+       >>   reverse(EVERY_CASE_TAC) >> fs[] >> rveq >> rename1 `_ _ decs = (n_state, ctors, res)` >>
+            imp_res_tac keep_Dlet >> rveq >> fs[Once evaluate_dec_def] >> EVERY_CASE_TAC >> fs[] >> 
+            rveq >> rw[UNION_EMPTY] >> 
+            `env with c updated_by $UNION {} = env` by fs[environment_component_equality] >> fs[]
+            >- (assume_tac evaluate_sing_notKeep_flat_state_rel >> fs[] >> pop_assum kall_tac >>
+                pop_assum (qspecl_then [`env`, `state'`, `new_state`, `Rerr e`, `x'`, 
+                    `reachable`, `removed_state`] mp_tac) >> rpt(disch_then drule) >> fs[]) 
+            >>  first_x_assum match_mp_tac >> fs[] >> asm_exists_tac >> fs[] >> 
+                imp_res_tac decsClosed_reduce >> fs[] >> assume_tac evaluate_sing_notKeep_flat_state_rel >> 
+                fs[] >> pop_assum kall_tac >>
+                pop_assum (qspecl_then [`env`, `state'`, `q`, `Rval [Conv NONE []]`, `x`, 
+                    `reachable`, `removed_state`] mp_tac) >> rpt(disch_then drule) >> fs[]
 
-        >- (
-            imp_res_tac keep_Dlet >> rveq >> fs[evaluate_dec_def] >>
-            Cases_on `evaluate (env with v :=[] ) state' [x]` >> fs[] >>
-            Cases_on `r` >> fs[] >>
 
-                EVERY_CASE_TAC >> fs[] >> rveq >>
-                `env with c updated_by $UNION {} = env` by fs[environment_component_equality] >>
-                fs[UNION_EMPTY] >>
-                first_x_assum match_mp_tac >> 
-                qexists_tac `q` >> fs[] >>
-                fs[flat_state_rel_def] >>
-                   
-                
-            
-            )
-        )
+);
 
-        >- (fs[evaluate_decs_def] >> `∃ r . evaluate_dec env removed_state h = r` by simp[] >> PairCases_on `r` >>
-            fs[] >> 
-            `r2 ≠ SOME (Rabort Rtype_error)` by (EVERY_CASE_TAC >> rveq >> fs[]
-            CCONTR_TAC >> fs[]) >> 
-            drule evaluate_dec_state_rel >> rpt (disch_then drule) >> rw[] >> fs[] >> Cases_on `r2` >> 
-            fs[] >> rw[] >> EVERY_CASE_TAC >> first_x_assum drule >> fs[] >> rveq >> disch_then drule >>
-            strip_tac >> fs[] >> rveq >> simp[]) 
-        >> reverse(EVERY_CASE_TAC) >> fs[] >> rveq >>
-           rename1 `_ = (s1, tn1, _)` >> rename1 `_ s1 ds = (s2, tn2, res)` >>
-           imp_res_tac keep_Dlet >> rveq
-            >- (fs[Once evaluate_dec_def] >> EVERY_CASE_TAC >> fs[] >> rveq >> rw[UNION_EMPTY] >>
-                drule keep_state_rel_thm >> disch_then drule >> disch_then drule >> fs[]) 
-            >> fs[Once evaluate_dec_def] >> EVERY_CASE_TAC >> fs[] >> rveq >> rw[UNION_EMPTY] >>
-               first_x_assum match_mp_tac >> qmatch_assum_abbrev_tac `evaluate_decs env2 _ _ = _` >>
-               `env2 = env` by (fs[flatSemTheory.environment_component_equality, Abbr `env2`]) >>
-               fs[] >> asm_exists_tac >> fs[] >> drule keep_state_rel_thm >> disch_then drule >>
-               disch_then drule >> fs[]
-*)
+
 (* in code, you can say get global -> in flatLang you have code in closures, which can get globals therefore
     -> therefore anything in which you can say "get global" must be in reachable set -> have to scan all closures and recclosures *)
 
@@ -216,7 +567,7 @@ val _ = export_theory();
 (*
 (**************************** STATE_REL *****************************)
 val state_rel_def = Define `
-    state_rel (reachable:num_set) s t ⇔ s.clock = t.clock ∧ s.refs = t.refs ∧ 
+    state_rel (reachable:num_set) (s:'ffi flatSem$state) t ⇔ s.clock = t.clock ∧ s.refs = t.refs ∧ 
     s.ffi = t.ffi ∧ LENGTH s.globals = LENGTH t.globals ∧ 
     ∀ n . n ∈ domain reachable ∧ n < LENGTH s.globals 
         ⇒  EL n s.globals = EL n t.globals
@@ -229,11 +580,6 @@ val evaluate_dec_state_rel = Q.store_thm("evaluate_dec_state_rel",
         result ≠ SOME (Rabort Rtype_error)
     ⇒ ∃ t1 . evaluate_dec env t h = (t1, new_ctors, result) ∧ 
         state_rel reachable s1 t1`,
-        rw[] >> 
-        Cases_on `h` >> fs[evaluate_dec_def] >>
-
-    (* TODO *)
-    
     cheat
 );
 
@@ -245,8 +591,8 @@ val evaluate_dec_state_rel = Q.store_thm("evaluate_dec_state_rel",
     ¬keep reachable h ∧ evaluate_dec env state h = (h1, new_ctors, result) ⇒ new_ctors = {}`,
     Cases_on `h` >> rw[keep_def] >> EVERY_CASE_TAC >> fs[] >>
     cheat
-    (* TODO *)
 );
+
 *)
 (* by running x, we don't do anything observable, so we can delete it 
     in particular can't write to any globals we care about
@@ -261,47 +607,16 @@ val not_keep_subterm = Q.store_thm("not_keep_subterm",
 
 
 val keep_state_rel_thm = Q.store_thm("keep_state_rel_thm",
-    `(∀ env (s:'ffi state) x s1 r reachable t . evaluate (env with v := []) s [x] = (s1, r) ∧ 
-        ¬keep reachable (Dlet x) ∧ state_rel reachable s t
-    
-    ⇒ state_rel reachable s1 t ∧ ∃ v . r = Rval [v]) ∧ 
-    
-`(∀env (s:'ffi flatSem$state) ls s' vs.
-      evaluate env s ls = (s',Rval vs) ⇒ LENGTH vs = LENGTH ls) ∧
-         (∀env (s:'ffi flatSem$state) v pes ev s' vs.
-               evaluate_match env s v pes ev = (s', Rval vs) ⇒ LENGTH vs = 1)`,
-    
-
-
-
-cheat);
-rw[]
-
-Induct >> fs[evaluate_def] >> rw[]
-
-
-
-imp_res_tac evaluate_sing
-evaluate_cons
-
-EVERY_CASE_TAC >>
-
-
-            rw[] >> qspecl_then [`reachable`, `(Raise t x)`, `x`, `t`] mp_tac not_keep_subterm >>
-            EVERY_CASE_TAC >> 
-            first_assum (qspecl_then [`t'`, `s1`, `s`, `reachable`, `env`, `r`] mp_tac) >> rw[] >>
-            first_assum (qspecl_then [`t'`, `q`, `s`, `reachable`, `env`, `Rval a`] mp_tac) >> rw[]
-             
-
-                  
-
->>    cheat
-);
+    `(∀ env (s:'ffi flatSem$state) x s1 r reachable t . evaluate (env with v := []) s [x] = (s1, r) ∧ 
+        ¬keep reachable (Dlet x) ∧ state_rel reachable s t    
+    ⇒ state_rel reachable s1 t ∧ ∃ v . r = Rval [v])`, 
+    cheat
+); 
 
 
 (***************************** REMOVAL *************************)
         
-        (* TODO - add assumption - if there is a get global in upcoming state, it is in reachable *)
+(* add assumption - if there is a get global in upcoming state, it is in reachable *)
 
 val removal_thm = Q.store_thm ("removal_thm",
     `∀ env s ds s1 new_ctors result ds1 t (reachable:num_set).
@@ -330,20 +645,6 @@ val removal_thm = Q.store_thm ("removal_thm",
                fs[] >> asm_exists_tac >> fs[] >> drule keep_state_rel_thm >> disch_then drule >>
                disch_then drule >> fs[]
 );
-
-
-      `(∀env (s:'ffi flatSem$state) ls s' vs.
-            evaluate env s ls = (s',Rval vs) ⇒ LENGTH vs = LENGTH ls) ∧
-    
-    `∀ env s ds s1 new_ctors result ds1 t (reachable:num_set).
-        flatSem$evaluate_decs env s ds = (s1, new_ctors, result) ∧
-        result ≠ SOME (Rabort Rtype_error) ∧
-        removeUnreachable reachable ds = ds1 ∧ state_rel reachable s t 
-    ⇒ ∃ t1 . 
-        flatSem$evaluate_decs env t ds1 = (t1, new_ctors, result) ∧
-        state_rel reachable s1 t1`,
-    
-    ho_match_mp_tac evaluate_ind
 *)
 
 (**************************** DLETS ******************************)
@@ -394,31 +695,9 @@ val count_GlobalVarInits_Dlet_def = Define `
 val one_Dlet_thm = Q.store_thm("one_Dlet_thm",
     `∀ e c p c1 ds d. source_to_flat$compile c p = (c1, ds) ∧ MEM d ds ∧ d = Dlet e 
     ⇒ count_GlobalVarInits e ≤ 1`,
-    (* TODO *)
     Induct_on `p`
     >-(rw[source_to_flatTheory.compile_def] >> fs[source_to_flatTheory.compile_decs_def] >>
        rw[] >> fs[] >> rw[count_GlobalVarInits_def] >> rw[dest_GlobalVarInit_def])
-    
-    
-    
-    >> rw[source_to_flatTheory.compile_def] >>
-    fs[source_to_flatTheory.compile_decs_def] >>
-    Cases_on `p` >>
-    >-(
-
-    Cases_on `h` >>
-    fs[source_to_flatTheory.compile_decs_def] >>
-    rw[] >> fs[] >>
-    rw[count_GlobalVarInits_def] >>
-    rw[dest_GlobalVarInit_def] >>
-
-
-    )
-   
-    rw[] >> fs[] >>
-    rw[Once count_GlobalVarInits_def] >>
-    rw[dest_GlobalVarInit_def] >>
-   
-    cheat
+    >> cheat
 );
 *)
